ground_zero/theorems/ua.lean
@@ -1,38 +1,39 @@
 import ground_zero.types.product
-open ground_zero.equiv (idtoeqv) ground_zero.not
-open ground_zero.equiv (homotopy)
-open ground_zero.structures
+open ground_zero.types.equiv (idtoeqv homotopy)
+open ground_zero.types.equiv (renaming id -> ideqv)
+open ground_zero.types.eq (renaming refl -> idp)
+open ground_zero.structures ground_zero.types.not
 
 namespace ground_zero
 
-local infix ` = ` := eq
+local infix ` = ` := types.eq
 universes u v
 
 axiom J {π : Π (α β : Sort u), α ≃ β → Sort v}
-  (h : Π (α : Sort u), π α α (equiv.id α))
+  (h : Π (α : Sort u), π α α (ideqv α))
   {α β : Sort u} (e : α ≃ β) : π α β e
 axiom Jβrule {π : Π (α β : Sort u), α ≃ β → Sort v}
-  {h : Π (α : Sort u), π α α (equiv.id α)} {α : Sort u} :
-  J h (equiv.id α) = h α :> π α α (equiv.id α)
+  {h : Π (α : Sort u), π α α (ideqv α)} {α : Sort u} :
+  J h (ideqv α) = h α :> π α α (ideqv α)
 
 noncomputable def ua {α β : Sort u} : α ≃ β → α = β :=
-J eq.refl
+J idp
 
 namespace ua
 
 noncomputable theorem comp_rule {α β : Sort u} (e : α ≃ β) :
   Π (x : α), x =[ua e] e.fst x := begin
   refine J _ e, intros γ x, simp [ua], transitivity,
-  apply eq.map (λ p, equiv.transport theorems.functions.idfun p x),
+  apply types.eq.map (λ p, types.equiv.transport theorems.functions.idfun p x),
   exact Jβrule, reflexivity
 end
 
 noncomputable theorem refl_on_ua {α : Sort u} :
-  ua (equiv.id α) = eq.refl α :=
+  ua (ideqv α) = idp α :=
 begin unfold ua, exact Jβrule end
 
 theorem idtoeqv_and_id {α : Sort u} :
-  idtoeqv (eq.refl α) = equiv.id α :=
+  idtoeqv (idp α) = ideqv α :=
 begin simp [idtoeqv] end
 
 noncomputable theorem prop_uniq {α β : Sort u} (p : α = β) :
@@ -51,26 +52,27 @@ noncomputable theorem univalence (α β : Sort u) :
 end
 
 def bool_to_universe : bool → Type
-| tt := ground_zero.unit
+| tt := types.unit
 | ff := empty
 
 theorem ff_neq_tt (h : ff = tt) : empty :=
-@ground_zero.eq.rec
+@ground_zero.types.eq.rec
   bool tt (λ b _, bool_to_universe b)
-  ground_zero.unit.star ff h⁻¹
+  types.unit.star ff h⁻¹
+
+def neg_bool_equiv : bool ≃ bool := begin
+  existsi bnot, split; existsi bnot; intro x; simp
+end
 
 noncomputable theorem universe_not_a_set : ¬(hset Type) :=
 begin
   intro error,
-  let e : bool ≃ bool := begin
-    existsi bnot, split; existsi bnot; intro x; simp
-  end,
-  let p : bool = bool := ua e,
-  let h := equiv.transport theorems.functions.idfun p tt,
-  let g : h = ff := comp_rule e tt,
+  let p : bool = bool := ua neg_bool_equiv,
+  let h := transport theorems.functions.idfun p tt,
+  let g : h = ff := comp_rule neg_bool_equiv tt,
   let oops : h = tt :=
-    (λ p, equiv.transport theorems.functions.idfun p tt) #
-    (@hset.intro _ error _ _ p (ground_zero.eq.refl bool)),
+    (λ p, transport theorems.functions.idfun p tt) #
+    (@hset.intro _ error _ _ p (idp bool)),
   let uh_oh : ff = tt := g⁻¹ ⬝ oops,
   apply ff_neq_tt, exact uh_oh
 end
@@ -90,23 +92,26 @@ begin
   reflexivity
 end
 
-theorem product_equiv₃ {α α' β β' : Sort u}
-  (e₁ : α ≃ α') (e₂ : β ≃ β') : (α × β) ≃ (α' × β') := begin
-  cases e₁ with f H, cases H with linv rinv,
-  cases linv with g α₁, cases rinv with h β₁,
-
-  cases e₂ with f' H, cases H with linv' rinv',
-  cases linv' with g' α₂, cases rinv' with h' β₂,
-
-  existsi (product.bimap f f'), split,
-  { existsi (product.bimap g g'), intro x,
-    cases x with u v, simp [*],
-    apply product.construction,
-    exact α₁ u, exact α₂ v },
-  { existsi (product.bimap h h'), intro x,
-    cases x with u v, simp [*],
-    apply product.construction,
-    exact β₁ u, exact β₂ v }
+section
+  open ground_zero.types.product
+  theorem product_equiv₃ {α α' β β' : Sort u}
+    (e₁ : α ≃ α') (e₂ : β ≃ β') : (α × β) ≃ (α' × β') := begin
+    cases e₁ with f H, cases H with linv rinv,
+    cases linv with g α₁, cases rinv with h β₁,
+  
+    cases e₂ with f' H, cases H with linv' rinv',
+    cases linv' with g' α₂, cases rinv' with h' β₂,
+  
+    existsi (bimap f f'), split,
+    { existsi (bimap g g'), intro x,
+      cases x with u v, simp [*],
+      apply construction,
+      exact α₁ u, exact α₂ v },
+    { existsi (bimap h h'), intro x,
+      cases x with u v, simp [*],
+      apply construction,
+      exact β₁ u, exact β₂ v }
+  end
 end
 
 theorem family_on_bool {π : bool → Sort u} :
